clightplus/compiler_proof/ClightPlus2ClightGenv.v
@@ -4,86 +4,86 @@ Require Import ModSem.
 Require Import ClightPlusExprgen ClightPlusgen ClightPlusSkel.
 
 Lemma in_get_fnsems_decomp clight_prog fn sk l i :
-NoDup (List.map fst l) ->
-alist_find fn (get_fnsems clight_prog sk l) = Some i ->
-exists f, i = cfunU (decomp_func sk (get_ce clight_prog) f) /\ alist_find fn l = Some (Gfun (Internal f)).
+  NoDup (List.map fst l) ->
+  alist_find fn (get_fnsems clight_prog sk l) = Some i ->
+  exists f, i = cfunU (decomp_func sk (get_ce clight_prog) f) /\ alist_find fn l = Some (Gfun (Internal f)).
 Proof.
-ginduction l; i; ss. des_ifs_safe. inv H. destruct g as [[f|? ? ? ?]|v].
-- ss. des_ifs; cycle 1. { apply IHl; et. } esplits; et.
-- hexploit IHl; et. i. des. esplits; et. des_ifs.
-    unfold rel_dec in Heq; ss. destruct dec; clarify.
-    apply alist_find_some in H1. eapply in_map with (f:=fst) in H1. ss.
-- hexploit IHl; et. i. des. esplits; et. des_ifs.
-    unfold rel_dec in Heq; ss. destruct dec; clarify.
-    apply alist_find_some in H1. eapply in_map with (f:=fst) in H1. ss.
+  ginduction l; i; ss. des_ifs_safe. inv H. destruct g as [[f|? ? ? ?]|v].
+  - ss. des_ifs; cycle 1. { apply IHl; et. } esplits; et.
+  - hexploit IHl; et. i. des. esplits; et. des_ifs.
+      unfold rel_dec in Heq; ss. destruct dec; clarify.
+      apply alist_find_some in H1. eapply in_map with (f:=fst) in H1. ss.
+  - hexploit IHl; et. i. des. esplits; et. des_ifs.
+      unfold rel_dec in Heq; ss. destruct dec; clarify.
+      apply alist_find_some in H1. eapply in_map with (f:=fst) in H1. ss.
 Qed.
 
 Lemma get_sk_nodup l t : get_sk l = Some t -> NoDup (List.map fst t).
 Proof.
-revert t. induction l; unfold get_sk; i; des_ifs; ss; cycle 2.
-{ apply IHl. unfold get_sk. ss. des_ifs. inv l0. exfalso. et. } { econs. }
-bsimpl. des. destruct a. ss. rewrite Heq0 in *. clear Heq0. ss.
-des_ifs. bsimpl. des. unfold chk_ident in Heq.
-rewrite forallb_app in Heq0. bsimpl. destruct Pos.eq_dec; clarify.
-clear Heq Heq1. rewrite list_norepet_app in l1. des. clear l2 l3.
-rewrite (List.map_map _ fst).
-replace (_ ∘ _) with (string_of_ident ∘ (@fst ident (globdef Clight.fundef type))).
-2:{ extensionalities. destruct H. ss. }
-rewrite <- (List.map_map _ string_of_ident).
-econs.
-- ii. apply n. apply in_map with (f:=ident_of_string) in H. rewrite <- e in H.
-    apply in_app. left. eassert (X: List.map fst (List.filter def_filter l) = _); [|rewrite X; et].
-    clear - Heq0. ginduction l; ss. i. des_ifs; ss; et.
-    bsimpl. des. unfold chk_ident in Heq0. destruct Pos.eq_dec; clarify. f_equal; et.
-- clear -Heq0 l1. ginduction l; i; ss. { econs. }
-    des_ifs; cycle 1. { apply IHl; et. }
-    inv l1. ss. bsimpl. des. econs; et.
-    ii. apply H1. apply in_map with (f:=ident_of_string) in H.
-    unfold chk_ident in Heq0. destruct Pos.eq_dec; clarify.
-    rewrite <- e in H.
-    eassert (X: List.map fst (List.filter def_filter l) = _); [|rewrite X; et].
-    clear - Heq1. induction l; i; ss.
-    des_ifs; et. ss. bsimpl. des. unfold chk_ident in Heq1. destruct Pos.eq_dec; clarify.
-    f_equal; et.
+  revert t. induction l; unfold get_sk; i; des_ifs. { econs. }
+  2:{ apply IHl. unfold get_sk. ss. des_ifs. ss. bsimpl. des. clarify. }
+  rewrite (List.map_map _ fst).
+  replace (_ ∘ _) with (string_of_ident ∘ (@fst ident (globdef Clight.fundef type))).
+  2:{ extensionalities. destruct H. ss. }
+  rewrite <- (List.map_map _ string_of_ident).
+  ss. des_ifs. econs.
+  - ss. ii. apply n. bsimpl. des. clear - Heq Heq0 Heq1 Heq3 Heq2 H.
+    move Heq3 at bottom. move Heq2 at bottom. revert_until Heq1. induction l; ss; i.
+    bsimpl. des. des_ifs; try tauto.
+    ss. des.
+    + left. bsimpl. des.
+      assert (ident_of_string (string_of_ident (fst a0)) = fst a0).
+      { unfold chk_ident in Heq2. des_ifs; ss; destruct Pos.eq_dec; clarify. }
+      assert (ident_of_string (string_of_ident (fst a)) = fst a).
+      { unfold chk_ident in Heq0. des_ifs; ss; destruct Pos.eq_dec; clarify. }
+      rewrite <- H0. rewrite <- H1. f_equal; et.
+    + right. bsimpl. des. apply IHl; et. 
+  - hexploit IHl. { ss. bsimpl. des. unfold get_sk. des_ifs. bsimpl. destruct list_norepet_dec; clarify. }
+    i. rewrite (List.map_map _ fst) in H.
+    replace (_ ∘ _) with (string_of_ident ∘ (@fst ident (globdef Clight.fundef type))) in H.
+    2:{ extensionalities. destruct H0. ss. }
+    rewrite List.map_map. et.
 Qed.
 
 Theorem in_tgt_prog_defs_decomp clight_prog mn md fn sk i :
-compile clight_prog mn = Some md ->
-alist_find fn (ModSem.fnsems (Mod.get_modsem md sk)) = Some i ->
-exists f, i = cfunU (decomp_func sk (get_ce clight_prog) f) /\ alist_find (ident_of_string fn) (prog_defs clight_prog) = Some (Gfun (Internal f)).
+  compile clight_prog mn = Some md ->
+  alist_find fn (ModSem.fnsems (Mod.get_modsem md sk)) = Some i ->
+  exists f, i = cfunU (decomp_func sk (get_ce clight_prog) f) /\ alist_find (ident_of_string fn) (prog_defs clight_prog) = Some (Gfun (Internal f)).
 Proof.
-unfold compile. i. des_ifs. ss.
-hexploit in_get_fnsems_decomp; et. { eapply get_sk_nodup; et. } 
-i. des. clarify. esplits; et.
-clear -Heq H1. revert_until clight_prog.
-generalize (prog_defs clight_prog).
-induction l; i; ss. { unfold get_sk in Heq. des_ifs. }
-unfold get_sk in Heq. destruct list_norepet_dec; clarify.
-destruct (_ && _) eqn: ?; clarify. bsimpl. des.
-des_ifs.
-- unfold def_filter in Heq0. ss. 
+  Local Opaque call_ban.
+  unfold compile. i. des_ifs. ss.
+  hexploit in_get_fnsems_decomp; et. { eapply get_sk_nodup; et. } 
+  i. des. clarify. esplits; et.
+  clear -Heq H1. revert_until clight_prog.
+  generalize (prog_defs clight_prog).
+  induction l; i; ss. { unfold get_sk in Heq. des_ifs. }
+  unfold get_sk in Heq. destruct list_norepet_dec; clarify.
+  destruct forallb eqn: ?; clarify. ss.
+  destruct (forallb chk_ident) eqn: ?; clarify. bsimpl. des.
+  des_ifs.
+  - unfold def_filter in Heq0.
     unfold rel_dec in Heq. ss. destruct dec; clarify. clear Heq.
     rewrite string_of_ident_of_string in H1.
     des_ifs; cycle 1.
     all: unfold rel_dec in Heq; ss; destruct dec; clarify.
-- exfalso.
-    hexploit IHl; et.
-    { ss. des_ifs. unfold get_sk. ss. des_ifs. inv l0. clarify. }
+  - exfalso.
+    hexploit IHl; et. { unfold get_sk. inv l0. des_ifs. destruct list_norepet_dec; clarify. }
     i. apply alist_find_some in H. apply in_map with (f:=fst) in H.
     unfold rel_dec in Heq. ss. destruct dec; clarify. clear Heq.
     inv l0. et.
-- ss. rewrite Heq0 in *. ss. bsimpl. des. unfold chk_ident in Heqb.
-    destruct Pos.eq_dec; clarify. rewrite e in *.
-    rewrite string_of_ident_of_string in *.
-    clear Heq0. des_ifs. { unfold rel_dec in *. ss. do 2 destruct dec; clarify. }
-    eapply IHl; et. unfold get_sk.
-    inv l0. des_ifs. ss. destruct list_norepet_dec; clarify.
-- eapply IHl; et. unfold get_sk. ss. rewrite Heq0 in *. inv l0.
-    des_ifs.
+  - simpl in Heqb0. bsimpl. des.
+    assert (ident_of_string (string_of_ident i) = i).
+    { unfold chk_ident in Heqb0. destruct Pos.eq_dec; clarify. }
+    clear Heqb Heq0. ss. des_ifs.
+    { unfold rel_dec in *. ss. do 2 destruct dec; clarify. }
+    eapply IHl; et. unfold get_sk. inv l0. des_ifs.
+    destruct list_norepet_dec; clarify.
+  - eapply IHl; et. unfold get_sk. inv l0. des_ifs.
+    destruct list_norepet_dec; clarify.
 Qed.
 
 Theorem in_tgt_prog_main clight_prog mn md :
-compile clight_prog mn = Some md -> prog_main clight_prog = ident_of_string "main".
+  compile clight_prog mn = Some md -> prog_main clight_prog = ident_of_string "main".
 Proof. unfold compile. des_ifs. Qed.
 
 Lemma tgt_genv_match_symb_def
@@ -95,8 +95,9 @@ Lemma tgt_genv_match_symb_def
 :
     gd1 = gd2.
 Proof.
-unfold compile, get_sk in COMP. des_ifs_safe. apply alist_find_some in INTGT.
-change (prog_defs clight_prog) with (AST.prog_defs clight_prog) in INTGT.
-hexploit prog_defmap_norepet; eauto; ss.
-i. apply Genv.find_def_symbol in H. des. clarify.
+  unfold compile, get_sk in COMP. des_ifs_safe. apply alist_find_some in INTGT.
+  change (prog_defs clight_prog) with (AST.prog_defs clight_prog) in INTGT.
+  bsimpl. des. destruct list_norepet_dec; clarify.
+  hexploit prog_defmap_norepet; eauto; ss.
+  i. apply Genv.find_def_symbol in H. des. clarify.
 Qed.
